kalloc/Verif_kalloc_kfree_examples.v
@@ -55,6 +55,36 @@ Definition kfree_kalloc_spec :=
 ).
 
 
+Definition kfree_kalloc_inverses_spec := 
+    DECLARE _kfree_kalloc
+    WITH gv:globals, sh : share, new_head:val, orig_head:val, xx:Z, ls:list val
+    PRE [ tptr tvoid ]
+        PROP(isptr new_head) 
+        PARAMS (new_head) GLOBALS(gv)
+        SEP (
+            KAF_globals gv  sh ls xx orig_head *
+            kalloc_token' KAF_APD sh (sizeof t_run) new_head
+        )
+    POST [ tptr tvoid ]
+        PROP( )
+        RETURN (new_head) (* we return the head like in the pop function*)
+        SEP (
+            KAF_globals gv sh ls xx orig_head *
+            kalloc_token' KAF_APD sh (sizeof t_run) new_head
+    ).
+
+
+Definition kalloc_kfree_inverses_spec : ident * funspec :=
+    DECLARE _kalloc_kfree
+    WITH sh : share, orig_head:val, xx:Z, ls:list val, gv:globals
+    PRE [ ] 
+        PROP () PARAMS() GLOBALS(gv) SEP (KAF_globals gv sh ls xx orig_head)
+    POST [ tvoid ] 
+        PROP ( ) RETURN () 
+        SEP (
+            KAF_globals gv sh ls xx orig_head
+        ).
+
 Definition kalloc_write_42_kfree_spec : ident * funspec :=
     DECLARE _kalloc_write_42_kfree
     WITH sh : share, orig_head:val, xx:Z, ls:list val, gv:globals
@@ -387,6 +417,37 @@ forward_call (kfree_spec_sub KAF_APD t_run) (new_head, gv, sh , ls, xx, orig_hea
             -- forward. Exists new_head. entailer. inversion H0; subst; entailer. unfold KAF_globals. entailer!. simplify_kalloc_token.
 Qed.
 
+Lemma body_kfree_kalloc_inverses: semax_body KAFVprog KAFGprog f_kfree_kalloc kfree_kalloc_inverses_spec.
+Proof.
+start_function.
+forward_call (kfree_spec_sub KAF_APD t_run) (new_head, gv, sh , ls, xx, orig_head). (* call kfree *)
+    + if_tac_auto_contradict.
+        *unfold KAF_globals. entailer!.
+        * unfold KAF_globals. entailer!. 
+            simplify_kalloc_token. 
+    + if_tac_auto_contradict.
+        *forward_call (kalloc_spec_sub KAF_APD t_run) (gv, sh , ls, xx, orig_head ). (* kalloc *)
+        if_tac; forward.
+        *forward_call (kalloc_spec_sub KAF_APD t_run) (gv, sh, orig_head::ls, xx, new_head ). (* kalloc *)
+        if_tac_auto_contradict; forward.
+        inversion H2; subst; entailer. unfold KAF_globals. entailer!. simplify_kalloc_token.
+Qed.
+
+Lemma body_kalloc_kfree_inverses: semax_body KAFVprog KAFGprog f_kalloc_kfree kalloc_kfree_inverses_spec.
+Proof.
+start_function.
+forward_call (kalloc_spec_sub KAF_APD t_run) (gv, sh , ls, xx, orig_head).
+- unfold KAF_globals. entailer!.
+- if_tac.
+    + forward_call (kfree_spec_sub KAF_APD t_run) (nullval, gv, sh , ls, xx, orig_head).
+        * if_tac_auto_contradict. entailer!.
+        * if_tac_auto_contradict. unfold KAF_globals. entailer!.
+    + Intros ab. assert_PROP(isptr orig_head).
+        * unfold type_kalloc_token. entailer!.
+        * forward_call (kfree_spec_sub KAF_APD t_run) (orig_head, gv, sh , snd ab, xx, fst ab).
+        -- if_tac_auto_contradict. entailer!.
+        -- if_tac_auto_contradict. unfold KAF_globals. entailer!.
+Qed.
 
 Lemma body_kalloc_write_42_kfree: semax_body KAFVprog KAFGprog f_kalloc_write_42_kfree kalloc_write_42_kfree_spec.
 Proof.
